feat: Add support for multiple return values (#1511)
This PR adds support for multiple return values in `Com`!

The core change is that `DialectSignature.outTy` now becomes
`DialectSignature.returnTypes`, and is generalized to return a List of
types. All the other changes are effectively the natural consequence of
this.

- The proof strategy in `Match.lean` has changed to rely more heavily on
Subtypes. This means that we can have simp lemmas that are effectively
keyed on the goals, instead of having to rely on remembering which
rewrite to apply (since they are disambiguated by side-condition).
- DCE had to be generalized to delete a (consecutive) range of variables
- We drive-by fix some printing instances so that (a) HVector's printing
no longer includes stray extra brackets and commas and (b) so that the
Com/Expr printing code does not include brackets/list-notation, but
instead look like, e.g., `(i64, i64)`
- The TermModel code got broken, but it's not actually used anywhere, so
:shrug:
- Finally, we adjust the entire rest of the project to align with the
possibility of multiple return values:
- Dialect operation semantics now have to return an hvector of values
(since there could be multiple); given that existing dialects only have
a single return for each operation, we just wrap the semantics in
`[...]\_h`
- Similarly, we have to introduce some list literals whenever a `Com` or
`Expr` type is referenced:
- There is also a `LeanMLIR.SingleReturnCompat` namespace which contains
backwards compatible aliasses, so for simple cases a straightforward fix
is `open LeanMLIR.SingleReturnCompat` to recover the old behaviour.
- Finally, we had to fix the proof automation to deal with the new shape
of semantics:
- In particular, I wrote `simpValuationApply`, which is a (d)simproc
that normalizes "applications of *fully-concrete* valuations to
*fully-concrete* variables", so for example, `(\empty ::\_v x ::\_v y)
\<1, _\>` is rewritten to just `x`.
- This used to be done by composing simp lemmas and hoping for the best;
this somehow broke but rather than figuring out why exactly moving to a
simproc gives us much more control and thus robustness

SSA/Core/ErasedContext.lean
@@ -496,17 +496,17 @@ def Hom.comp : Hom Γ Ξ :=
 end Comp
 
 /--
-  `map.with v₁ v₂` adjusts a single variable of a Context map, so that in the resulting map
-   * `v₁` now maps to `v₂`
+  `map.with v₁ v₂` adjusts a vector of variables of a Context map, so that in
+  the resulting map:
+   * `v₁[i]` now maps to `v₂[i]`
    * all other variables `v` still map to `map v` as in the original map
 -/
-def Hom.with [DecidableEq Ty] {Γ₁ Γ₂ : Ctxt Ty} (f : Γ₁.Hom Γ₂) {t : Ty}
-    (v₁ : Γ₁.Var t) (v₂ : Γ₂.Var t) : Γ₁.Hom Γ₂ :=
-  fun t' w =>
-    if h : ∃ ty_eq : t = t', ty_eq ▸ w = v₁ then
-      v₂.cast h.fst
-    else
-      f w
+def Hom.with [DecidableEq Ty] {Γ₁ Γ₂ : Ctxt Ty} (f : Γ₁.Hom Γ₂) {ts}
+    (v₁ : HVector Γ₁.Var ts) (v₂ : HVector Γ₂.Var ts) : Γ₁.Hom Γ₂ :=
+  fun _ w =>
+    match v₁.idxOf? w with
+    | none => f w
+    | some ⟨i, h⟩ => (v₂.get i).cast h
 
 def Hom.snocMap {Γ Γ' : Ctxt Ty} (f : Hom Γ Γ') {t : Ty} :
     (Γ.snoc t).Hom (Γ'.snoc t) := by
@@ -793,26 +793,39 @@ def Valuation.comap {Γi Γo : Ctxt Ty} (Γiv: Γi.Valuation) (hom : Ctxt.Hom Γ
 /-! ### Reassign Variables-/
 
 /-- Reassign the variable var to value val in context ctxt -/
-def Valuation.reassignVar [DecidableEq Ty] {t : Ty} {Γ : Ctxt Ty}
-    (V : Γ.Valuation) (var : Var Γ t) (val : toType t) : Γ.Valuation :=
-  fun tneedle vneedle =>
-    if h : ∃ h : t = tneedle, h ▸ vneedle = var
-    then h.fst ▸ val
-    else V vneedle
+def Valuation.reassignVars [DecidableEq Ty] {ts : List Ty} {Γ : Ctxt Ty}
+    (V : Γ.Valuation) (var : HVector Γ.Var ts) (val : HVector toType ts) : Γ.Valuation :=
+  fun _ vneedle =>
+    match var.idxOf? vneedle with
+    | none => V vneedle
+    | some ⟨i, h⟩ => h ▸ val.get i
 
-@[simp] lemma Valuation.reassignVar_eq [DecidableEq Ty] (V : Γ.Valuation) :
-    V.reassignVar v (V v) = V := by
-  funext t v
-  simp only [reassignVar, dite_eq_right_iff, forall_exists_index]
-  rintro rfl rfl
-  rfl
+@[simp] lemma Valuation.reassignVars_eq [DecidableEq Ty] (V : Γ.Valuation) :
+    V.reassignVars vs (vs.map V) = V := by
+  funext t w
+  unfold reassignVars
+  induction vs
+  case nil => rfl
+  case cons v vs ih =>
+    by_cases h_eq : w.eq v
+    · have := h_eq.ty_eq
+      subst this
+      have := h_eq.to_eq
+      subst this
+      simp
+    · unfold Var.eq at h_eq
+      simp only [HVector.idxOf?, h_eq, ↓reduceDIte, List.get_eq_getElem, List.length_cons,
+        HVector.map_cons]
+      split at ih <;> simp_all
 
 @[simp] lemma Valuation.comap_with [DecidableEq Ty] {Γ Δ : Ctxt Ty}
-    {Γv : Valuation Γ} {map : Δ.Hom Γ} {v : Var Δ ty} {w : Var Γ ty} :
-    Γv.comap (map.with v w) = (Γv.comap map).reassignVar v (Γv w) := by
+    {V : Valuation Γ} {map : Δ.Hom Γ} {vs : HVector Δ.Var ty} {ws : HVector Γ.Var ty} :
+    V.comap (map.with vs ws) = (V.comap map).reassignVars vs (ws.map V) := by
   funext t' v'
-  simp only [comap, Hom.with, reassignVar]
-  split_ifs <;> aesop
+  simp only [comap, Hom.with, reassignVars]
+  split <;> aesop
+
+/-! ### Recursion -/
 
 /-- Recursion principle for valuations in terms of `Valuation.nil` and `Valuation.snoc` -/
 @[elab_as_elim, induction_eliminator]
@@ -834,17 +847,6 @@ def Valuation.cast {Γ Δ : Ctxt Ty} (h : Γ = Δ) (V : Valuation Γ) : Valuatio
 
 @[simp] lemma Valuation.cast_apply {Γ : Ctxt Ty} (h : Γ = Δ) (V : Γ.Valuation) (v : Δ.Var t) :
     V.cast h v = V (v.castCtxt h.symm) := rfl
-
-/-- reassigning a variable to the same value that has been looked up is identity. -/
-theorem Valuation.reassignVar_eq_of_lookup [DecidableEq Ty]
-    {Γ : Ctxt Ty} {V : Γ.Valuation} {var : Var Γ t} :
-    (V.reassignVar var (V var)) = V := by
-  funext t' v
-  simp only [reassignVar, dite_eq_right_iff, forall_exists_index]
-  intros h x
-  subst h
-  subst x
-  rfl
 
 /-- Show that a valuation is equivalent to a `HVector` -/
 def Valuation.equivHVector {Γ : List Ty} : Valuation ⟨Γ⟩ ≃ HVector toType Γ where
