SSA/Core/Framework.lean
@@ -14,6 +14,7 @@ import Mathlib.Data.Finset.Piecewise
 set_option deprecated.oldSectionVars true
 
 theorem Id.pure_eq' (a : α) : (pure a : Id α) = a := rfl
+theorem Id.map_eq' (x : Id α) (f : α → β) : f <$> x = f x := rfl
 theorem Id.bind_eq' (x : Id α) (f : α → id β) : x >>= f = f x := rfl
 
 open Ctxt (Var VarSet Valuation Hom)
@@ -64,39 +65,40 @@ theorem _root_.Pure.pure_cast {f} [inst : Pure f] (b : β) (h : β = α) :
 
 /- # Classes -/
 
-abbrev RegionSignature Ty := List (Ctxt Ty × Ty)
+abbrev RegionSignature Ty := List (Ctxt Ty × List Ty)
 
 structure Signature (Ty : Type) where
   mkEffectful ::
-  sig        : List Ty
-  regSig     : RegionSignature Ty
-  outTy      : Ty
-  effectKind : EffectKind := .pure
+  sig         : List Ty
+  regSig      : RegionSignature Ty
+  returnTypes : List Ty
+  effectKind  : EffectKind := .pure
 
-abbrev Signature.mk (sig : List Ty) (regSig : RegionSignature Ty) (outTy : Ty) : Signature Ty :=
- { sig := sig, regSig := regSig, outTy := outTy }
+abbrev Signature.mk (sig : List Ty) (regSig : RegionSignature Ty) (returnTypes : List Ty) : Signature Ty :=
+ { sig, regSig, returnTypes }
 
 class DialectSignature (d : Dialect) where
   signature : d.Op → Signature d.Ty
 export DialectSignature (signature)
 
-section
+namespace DialectSignature
 variable {d} [s : DialectSignature d]
 
-def DialectSignature.sig        := Signature.sig ∘ s.signature
-def DialectSignature.regSig     := Signature.regSig ∘ s.signature
-def DialectSignature.outTy      := Signature.outTy ∘ s.signature
-def DialectSignature.effectKind := Signature.effectKind ∘ s.signature
+def sig          := Signature.sig ∘ s.signature
+def regSig       := Signature.regSig ∘ s.signature
+def returnTypes  := Signature.returnTypes ∘ s.signature
+def effectKind   := Signature.effectKind ∘ s.signature
 
-end
-
+end DialectSignature
 
 class DialectDenote (d : Dialect) [TyDenote d.Ty] [DialectSignature d] where
   denote : (op : d.Op) → HVector toType (DialectSignature.sig op) →
-    (HVector (fun t : Ctxt d.Ty × d.Ty => t.1.Valuation
-      → EffectKind.impure.toMonad d.m (toType t.2))
+    (HVector (fun t : Ctxt d.Ty × List d.Ty =>
+      t.1.Valuation
+      → EffectKind.impure.toMonad d.m (HVector toType t.2))
             (DialectSignature.regSig op)) →
-    ((DialectSignature.effectKind op).toMonad d.m (toType <| DialectSignature.outTy op))
+    ((DialectSignature.effectKind op).toMonad d.m
+      (HVector toType <| DialectSignature.returnTypes op))
 
 /-
 Some considerations about purity:
@@ -153,9 +155,9 @@ class ToPrint (d : Dialect) where
   /-- Prints the name of the dialect. -/
   printDialect : String
   /-- Prints the return instruction of the dialect. -/
-  printReturn : d.Ty → String
+  printReturn : List d.Ty → String
   /-- Prints the function header of the dialect. -/
-  printFunc : d.Ty → String
+  printFunc : List d.Ty → String
 
 /- # Datastructures -/
 section DataStructures
@@ -164,34 +166,44 @@ variable (d : Dialect) [DialectSignature d]
 
 mutual
 /-- An intrinsically typed expression whose effect is *at most* EffectKind -/
-inductive Expr : (Γ : Ctxt d.Ty) → (eff : EffectKind) → (ty : d.Ty) → Type where
+inductive Expr : (Γ : Ctxt d.Ty) → (eff : EffectKind) → (ty : List d.Ty) → Type where
   | mk {Γ} {ty} (op : d.Op)
-    (ty_eq : ty = DialectSignature.outTy op)
+    (ty_eq : ty = DialectSignature.returnTypes op)
     (eff_le : DialectSignature.effectKind op ≤ eff)
     (args : HVector (Var Γ) <| DialectSignature.sig op)
     /- For now, assume that regions are impure.
        We keep it this way to minimize the total amount of disruption in our definitions.
        We shall change this once the rest of the file goes through. -/
-    (regArgs : HVector (fun t : Ctxt d.Ty × d.Ty => Com t.1 .impure t.2)
+    (regArgs : HVector (fun t : Ctxt d.Ty × List d.Ty => Com t.1 .impure t.2)
       (DialectSignature.regSig op)) : Expr Γ eff ty
-
 
 /-- A very simple intrinsically typed program: a sequence of let bindings.
 Note that the `EffectKind` is uniform: if a `Com` is `pure`, then the expression
 and its body are pure, and if a `Com` is `impure`, then both the expression and
 the body are impure!
 -/
-inductive Com : Ctxt d.Ty → EffectKind → d.Ty → Type where
-  | ret {eff : EffectKind} (v : Var Γ t) : Com Γ eff t
-  | var (e : Expr Γ eff α) (body : Com (Γ.snoc α) eff β) : Com Γ eff β
+inductive Com : Ctxt d.Ty → EffectKind → List d.Ty → Type where
+  | rets {Γ} {tys} {eff : EffectKind} (vs : HVector Γ.Var tys) : Com Γ eff tys
+  | var (e : Expr Γ eff ty) (body : Com (Γ ++ ty) eff β) : Com Γ eff β
 end
+
+/-! ### `Expr` output context -/
+/-- The context immediately *after* this expression. -/
+abbrev Expr.outContext (_ : Expr d Γ eff ts) : Ctxt d.Ty :=
+  Γ ++ ts
+
+/-! ### Regions -/
+abbrev Regions (regSig : RegionSignature d.Ty) : Type :=
+  HVector (fun t => Com d t.1 .impure t.2) regSig
+
+/-! ### Lets -/
 
 /-- `Lets d Γ_in Γ_out` is a sequence of lets which are well-formed under
 context `Γ_out` and result in context `Γ_in`. -/
 inductive Lets (Γ_in : Ctxt d.Ty) (eff : EffectKind) :
     (Γ_out : Ctxt d.Ty) → Type where
   | nil : Lets Γ_in eff Γ_in
-  | var (body : Lets Γ_in eff Γ_out) (e : Expr d Γ_out eff t) : Lets Γ_in eff (Γ_out.snoc t)
+  | var (body : Lets Γ_in eff Γ_out) (e : Expr d Γ_out eff t) : Lets Γ_in eff e.outContext
 
 /-! ### DecidableEq instance -/
 --TODO: this should be derived later on when a derive handler is implemented
@@ -200,7 +212,7 @@ mutual -- DecEq
 variable {d} [DialectSignature d]
 
 protected instance HVector.decidableEqReg [DecidableEq d.Op] [DecidableEq d.Ty] :
-    ∀ {l : List (Ctxt d.Ty × d.Ty)}, DecidableEq (HVector (fun t => Com d t.1 .impure t.2) l)
+    ∀ {l : RegionSignature d.Ty}, DecidableEq (HVector (fun t => Com d t.1 .impure t.2) l)
   | _, .nil, .nil => isTrue rfl
   | _, .cons x₁ v₁, .cons x₂ v₂ =>
     letI := HVector.decidableEqReg v₁ v₂
@@ -208,10 +220,9 @@ protected instance HVector.decidableEqReg [DecidableEq d.Op] [DecidableEq d.Ty] 
     decidable_of_iff (x₁ = x₂ ∧ v₁ = v₂) (by simp)
 
 protected instance Expr.decidableEq [DecidableEq d.Op] [DecidableEq d.Ty] :
-    {Γ : Ctxt d.Ty} → {ty : d.Ty} → DecidableEq (Expr d Γ eff ty)
-  | _, _, .mk op₁ rfl eff_le₁ arg₁ regArgs₁, .mk op₂ eq eff_le₂ arg₂ regArgs₂ =>
-    if ho : op₁ = op₂
-    then by
+    {Γ : Ctxt d.Ty} → {ty : List d.Ty} → DecidableEq (Expr d Γ eff ty)
+  | Γ, _, .mk op₁ rfl eff_le₁ arg₁ regArgs₁, .mk op₂ eq eff_le₂ arg₂ regArgs₂ =>
+    if ho : op₁ = op₂ then by
       subst ho
       letI := HVector.decidableEq arg₁ arg₂
       letI := HVector.decidableEqReg regArgs₁ regArgs₂
@@ -219,18 +230,18 @@ protected instance Expr.decidableEq [DecidableEq d.Op] [DecidableEq d.Ty] :
     else isFalse (by simp_all)
 
 protected instance Com.decidableEq [DecidableEq d.Op] [DecidableEq d.Ty]
-    {Γ : Ctxt d.Ty} {eff : EffectKind} {ty : d.Ty} : DecidableEq (Com d Γ eff ty)
-  | .ret v₁, .ret v₂ => decidable_of_iff (v₁ = v₂) (by simp)
-  | .var (α := α₁) e₁ body₁, .var (α := α₂) e₂ body₂ =>
-    if hα : α₁ = α₂
+    {Γ : Ctxt d.Ty} {eff : EffectKind} {tys : List d.Ty} : DecidableEq (Com d Γ eff tys)
+  | .rets v₁, .rets v₂ => decidable_of_iff (v₁ = v₂) (by simp)
+  | .var (ty := ty₁) e₁ body₁, .var (ty := ty₂) e₂ body₂ =>
+    if hα : ty₁ = ty₂
     then by
       subst hα
       letI := Expr.decidableEq e₁ e₂
       letI := Com.decidableEq body₁ body₂
       exact decidable_of_iff (e₁ = e₂ ∧ body₁ = body₂) (by simp)
     else isFalse (by simp_all)
-  | .ret _, .var _ _ => isFalse (fun h => Com.noConfusion h)
-  | .var _ _, .ret _ => isFalse (fun h => Com.noConfusion h)
+  | .rets _, .var _ _ => isFalse (fun h => Com.noConfusion h)
+  | .var _ _, .rets _ => isFalse (fun h => Com.noConfusion h)
 
 end -- decEq
 
@@ -242,31 +253,27 @@ end DataStructures
 
 variable {d : Dialect} [DialectSignature d]
 
-
-/-!
-### `Expr` output context
--/
-
-/-- The context immediately *after* this expression. -/
-abbrev Expr.outContext (_ : Expr d Γ eff t) : Ctxt d.Ty :=
-  Γ.snoc t
-
 /-!
 ### Com recursors
 -/
 
 section Rec
 variable {eff t} {motive : ∀ {Γ}, Com d Γ eff t → Sort u}
-          (ret : ∀ {Γ} , (v : Var Γ t) → motive (Com.ret v))
-          (var : ∀ {Γ} {u : d.Ty},
+          (rets : ∀ {Γ : Ctxt _} , (v : HVector Γ.Var t) → motive (Com.rets v))
+          (var : ∀ {Γ} {u},
             (e : Expr d Γ eff u) → (body : Com d e.outContext eff t) →
               motive body → motive (Com.var e body))
 
 @[elab_as_elim]
 def Com.recAux' {Γ} : (com : Com d Γ eff t) → motive com
-  | Com.ret v => ret v
+  | Com.rets v => rets v
   | Com.var e body => var e body (Com.recAux' body)
 
+/--
+`Com.rec'` is a simple recursor for `Com` -- meaning it does not facilitate
+mutual recursion on the contained expressions or regions. In return, it has
+nicer def-eqs than a pattern-match based definition would.
+-/
 @[implemented_by Com.recAux', elab_as_elim, induction_eliminator]
 -- ^^^^ `Com.rec` is noncomputable, so have a computable version as well
 --      See `Com.recAux'_eq` for a theorem that states these definitions are equal
@@ -279,8 +286,8 @@ def Com.rec' {Γ} (com : Com d Γ eff t) : motive com :=
       (h₁ : eff = eff') → (h₂ : t = t') → motive (h₁ ▸ h₂ ▸ c))
     (motive_3 := fun _ _ => PUnit)
     (fun _ _ _ _ _ _ => ⟨⟩) -- `Expr.mk` case
-    (fun v h₁ h₂ => -- `Com.ret` case
-      cast (by subst h₁ h₂; rfl) <| ret (h₂ ▸ v))
+    (fun v h₁ h₂ => -- `Com.rets` case
+      cast (by subst h₁ h₂; rfl) <| rets (h₂ ▸ v))
     (fun e' body' _ r' h₁ h₂ => -- `Com.var` case
       let e := h₁ ▸ e'
       let body : Com _ _ eff t := cast (by simp_all) body'
@@ -292,66 +299,67 @@ def Com.rec' {Γ} (com : Com d Γ eff t) : motive com :=
     rfl
     rfl
 
-variable {ret} {var}
+variable {rets} {var} {Γ : Ctxt _}
 
-@[simp] lemma Com.rec'_ret (v : Var Γ t) :
-    (Com.ret (d:=d) (eff := eff) v).rec' (motive:=motive) ret var = ret v :=
+@[simp] lemma Com.rec'_rets (v : HVector Γ.Var t) :
+    (Com.rets (d:=d) (eff := eff) v).rec' (motive:=motive) rets var = rets v :=
   rfl
 
 @[simp] lemma Com.rec'_var (e : Expr d Γ eff u) (body : Com d _ _ t) :
-    (Com.var e body).rec' (motive:=motive) ret var
-    = var e body (body.rec' (motive:=motive) ret var) :=
+    (Com.var e body).rec' (motive:=motive) rets var
+    = var e body (body.rec' (motive:=motive) rets var) :=
   rfl
 
-omit ret var in
+omit rets var in
 theorem Com.recAux'_eq :
     Com.recAux' (motive:=motive) = Com.rec' (motive:=motive) := by
-  funext ret var Γ com
+  funext rets var Γ com
   induction com <;> simp [recAux', *]
 
 end Rec
 
-def Expr.op {Γ : Ctxt d.Ty} {eff : EffectKind} {ty : d.Ty} (e : Expr d Γ eff ty) : d.Op :=
+def Expr.op {Γ : Ctxt d.Ty} {eff : EffectKind} {ty} (e : Expr d Γ eff ty) : d.Op :=
   Expr.casesOn e (fun op _ _ _ _ => op)
 
-theorem Expr.eff_le {Γ : Ctxt d.Ty} {ty : d.Ty} (e : Expr d Γ eff ty) :
+theorem Expr.eff_le {Γ : Ctxt d.Ty} {ty} (e : Expr d Γ eff ty) :
   DialectSignature.effectKind e.op ≤ eff :=
   Expr.casesOn e (fun _ _ eff_le _ _ => eff_le)
 
-theorem Expr.ty_eq {Γ : Ctxt d.Ty} {ty : d.Ty} (e : Expr d Γ eff ty) :
-    ty = DialectSignature.outTy e.op :=
+theorem Expr.ty_eq {Γ : Ctxt d.Ty} {tys : List d.Ty} (e : Expr d Γ eff tys) :
+    tys = DialectSignature.returnTypes e.op :=
   Expr.casesOn e (fun _ ty_eq _ _ _ => ty_eq)
 
-def Expr.args {Γ : Ctxt d.Ty} {ty : d.Ty} (e : Expr d Γ eff ty) :
+def Expr.args {Γ ts} (e : Expr d Γ eff ts) :
     HVector (Var Γ) (DialectSignature.sig e.op) :=
   Expr.casesOn e (fun _ _ _ args _ => args)
 
-def Expr.regArgs {Γ : Ctxt d.Ty} {ty : d.Ty} (e : Expr d Γ eff ty) :
-    HVector (fun t : Ctxt d.Ty × d.Ty => Com d t.1 .impure t.2) (DialectSignature.regSig e.op) :=
+def Expr.regArgs {Γ ts} (e : Expr d Γ eff ts) :
+    Regions d (DialectSignature.regSig e.op) :=
   Expr.casesOn e (fun _ _ _ _ regArgs => regArgs)
 
-/-- `e.returnVar` is the variable in `e.outContext` which is bound by `e`. -/
-def Expr.returnVar (e : Expr d Γ eff ty) : e.outContext.Var ty :=
-  Var.last _ _
+/-- `e.returnVars` is the vector of variables in `e.outContext` which are bound by `e`. -/
+def Expr.returnVars (e : Expr d Γ eff tys) : HVector e.outContext.Var tys :=
+  .ofFn _ _ <| fun i => (Var.ofFin i).appendInr
 
 /-! Projection equations for `Expr` -/
 @[simp]
-theorem Expr.op_mk {Γ : Ctxt d.Ty} {ty : d.Ty} {eff : EffectKind} (op : d.Op)
-    (ty_eq : ty = DialectSignature.outTy op)
+theorem Expr.op_mk {Γ : Ctxt d.Ty} {ty} {eff : EffectKind} (op : d.Op)
+    (ty_eq : ty = DialectSignature.returnTypes op)
     (eff_le : DialectSignature.effectKind op ≤ eff)
-    (args : HVector (Var Γ) (DialectSignature.sig op)) (regArgs):
+    (args : HVector (Var Γ) (DialectSignature.sig op))
+    (regArgs) :
     (Expr.mk op ty_eq eff_le args regArgs).op = op := rfl
 
 @[simp]
-theorem Expr.args_mk {Γ : Ctxt d.Ty} {ty : d.Ty} {eff : EffectKind} (op : d.Op)
-    (ty_eq : ty = DialectSignature.outTy op)
+theorem Expr.args_mk {Γ : Ctxt d.Ty} {ty eff op}
+    (ty_eq : ty = DialectSignature.returnTypes op)
     (eff_le : DialectSignature.effectKind op ≤ eff)
     (args : HVector (Var Γ) (DialectSignature.sig op)) (regArgs) :
     (Expr.mk op ty_eq eff_le args regArgs).args = args := rfl
 
 @[simp]
-theorem Expr.regArgs_mk {Γ : Ctxt d.Ty} {ty : d.Ty} {eff : EffectKind} (op : d.Op)
-    (ty_eq : ty = DialectSignature.outTy op)
+theorem Expr.regArgs_mk {Γ : Ctxt d.Ty} {ty eff op}
+    (ty_eq : ty = DialectSignature.returnTypes op)
     (eff_le : DialectSignature.effectKind op ≤ eff)
     (args : HVector (Var Γ) (DialectSignature.sig op)) (regArgs) :
     (Expr.mk op ty_eq eff_le args regArgs).regArgs = regArgs := rfl
@@ -363,13 +371,40 @@ theorem Expr.regArgs_mk {Γ : Ctxt d.Ty} {ty : d.Ty} {eff : EffectKind} (op : d.
 /-- The size of a `Com` is given by the number of let-bindings it contains -/
 def Com.size : Com d Γ eff t → Nat :=
   Com.rec'
-    /- ret _ -/       (fun _ => 0)
+    /- rets _ -/       (fun _ => 0)
     /- var _ body -/ (fun _ _body bodySize => bodySize + 1)
 
-section Lemmas
+@[simp, grind=] def Expr.bvars (e : Expr d Γ eff Δ) : Nat :=
+  (DialectSignature.returnTypes e.op).length
 
-@[simp] lemma Com.size_ret  : (ret v : Com d Γ eff t).size = 0 := rfl
-@[simp] lemma Com.size_var : (var e body : Com d Γ eff t).size = body.size + 1 := rfl
+/-- The number of variables bound in a `Com`. This is related to the `size`, but
+will differ in the presence of let-bindings with multiple return variables.
+
+NOTE: this ignores any regions. -/
+def Com.bvars : Com d Γ eff t → Nat :=
+  Com.rec'
+    /- rets _ -/      (fun _ => 0)
+    /- var e body -/ (fun e _body bodySize => e.bvars + bodySize)
+
+section Lemmas
+namespace Com
+
+@[simp] lemma size_rets  : (rets v : Com d Γ eff t).size = 0 := rfl
+@[simp] lemma size_var : (var e body : Com d Γ eff t).size = body.size + 1 := rfl
+
+@[simp] lemma bvars_rets  : (rets v : Com d Γ eff t).bvars = 0 := rfl
+@[simp] lemma bvars_var  :
+  (var e body : Com d Γ eff t).bvars = e.bvars + body.bvars := rfl
+
+end Com
+
+@[simp] lemma Ctxt.get_add_bvars (e : Expr d Γ eff ts) (i : Nat) :
+    e.outContext[i + e.bvars]? = Γ[i]? := by
+  rcases e with ⟨op, rfl, _, _⟩
+  rcases Γ
+  simp only [ofList_append, Expr.bvars, Expr.op_mk, getElem?_ofList]
+  rw [List.getElem?_append_right (by simp)]
+  grind
 
 end Lemmas
 
@@ -379,55 +414,58 @@ end Lemmas
 
 /-- The `outContext` of a program is a context which includes variables for all let-bindings
 of the program. That is, it is the context under which the return value is typed -/
-def Com.outContext {Γ} : Com d Γ eff t → Ctxt d.Ty :=
+def Com.outContext {Γ} : Com d Γ eff ts → Ctxt d.Ty :=
   Com.rec' (motive := fun _ => Ctxt d.Ty)
-    (@fun Γ _ => Γ) -- `Com.ret` case
+    (@fun Γ _ => Γ) -- `Com.rets` case
     (fun _ _ r => r) -- `Com.var` case
 
 /-- The difference between the context `Γ` under which `com` is typed, and the output context of
 that same `com` -/
-def Com.outContextDiff (com : Com d Γ eff t) : Γ.Diff com.outContext :=
-  ⟨com.size, by
+def Com.outContextDiff (com : Com d Γ eff ts) : Γ.Diff com.outContext :=
+  ⟨com.bvars, by
     intro i t h;
     unfold outContext
     induction com generalizing i
-    case ret => exact h
-    case var ih =>
-      rw [rec'_var, size_var, ← Nat.add_assoc, Nat.add_comm _ 1, ← Nat.add_assoc, ih]
-      simpa [Ctxt.snoc, Nat.add_comm 1 _] using h⟩
+    case rets => exact h
+    case var e _ ih =>
+      simp only [rec'_var, bvars_var]
+      rw [← Nat.add_assoc]
+      apply ih
+      rw [Ctxt.get_add_bvars e, h]⟩
 
 /-- `com.outContextHom` is the canonical homorphism from free variables of `com` to those same
 variables in the output context of `com` -/
 def Com.outContextHom (com : Com d Γ eff t) : Γ.Hom com.outContext :=
   com.outContextDiff.toHom
 
-/-- The return variable of a program -/
-def Com.returnVar : (com : Com d Γ eff t) → Var com.outContext t
-  | .ret v => v
-  | .var _ body => body.returnVar
+/-- The return variables of a program -/
+def Com.returnVars : (com : Com d Γ eff ts) → HVector (Var com.outContext) ts
+  | .rets vs => vs
+  | .var _ body => body.returnVars
 
-@[simp] def Expr.contextHom (e : Expr d Γ eff ts) : Γ.Hom e.outContext :=
-  @fun _ => Var.toSnoc
+abbrev Expr.contextHom (e : Expr d Γ eff ts) : Γ.Hom e.outContext :=
+  Hom.id.appendCodomain
 
 section Lemmas
 
-@[simp] lemma Com.outContext_ret (v : Var Γ t) : (ret v : Com d Γ eff t).outContext = Γ := rfl
-@[simp] lemma Com.outContext_var {eff} (e : Expr d Γ eff t) (body : Com d (Γ.snoc t) eff u) :
+@[simp] lemma Com.outContext_rets (vs : HVector Γ.Var t) : (rets vs : Com d Γ eff t).outContext = Γ := rfl
+@[simp] lemma Com.outContext_var {eff} (e : Expr d Γ eff t) (body : Com d e.outContext eff u) :
     (Com.var e body).outContext = body.outContext := rfl
 
-@[simp] lemma Com.outContextHom_ret (v : Var Γ t) :
-    (ret v : Com d Γ eff t).outContextHom = Ctxt.Hom.id := rfl
+@[simp] lemma Com.outContextHom_rets (v : HVector Γ.Var t) :
+    (rets v : Com d Γ eff t).outContextHom = Ctxt.Hom.id := rfl
 @[simp] lemma Com.outContextHom_var :
-    (var e body : Com d Γ eff t).outContextHom = body.outContextHom.unSnoc := by
-  funext t' v'
-  simp only [outContext_var, outContextHom, Ctxt.Diff.toHom, Ctxt.Diff.Valid, outContextDiff,
-    size_var, Ctxt.Hom.unSnoc, Var.val_toSnoc]
-  ac_rfl
+    (var e body : Com d Γ eff t).outContextHom
+    = e.contextHom.comp body.outContextHom := by
+  funext t v
+  apply Subtype.eq
+  simp [outContextHom, outContextDiff, Expr.contextHom, Ctxt.Hom.comp, Expr.bvars,
+    e.ty_eq]
+  omega
 
-@[simp] lemma Com.returnVar_ret : returnVar (ret v : Com d Γ eff t) = v := by simp [returnVar]
-@[simp] lemma Com.returnVar_var :
-    returnVar (var (d:=d) (eff:=eff) e body) = body.returnVar := by
-  simp [returnVar]
+@[simp] lemma Com.returnVars_rets : returnVars (rets vs : Com d Γ eff t) = vs := rfl
+@[simp] lemma Com.returnVars_var :
+    returnVars (var (d:=d) (eff:=eff) e body) = body.returnVars := rfl
 
 end Lemmas
 
@@ -440,21 +478,22 @@ variable [TyDenote d.Ty] [DialectDenote d] [DecidableEq d.Ty] [Monad d.m] [Lawfu
 mutual
 
 def HVector.denote :
-    {l : List (Ctxt d.Ty × d.Ty)} → (T : HVector (fun t => Com d t.1 .impure t.2) l) →
-    HVector (fun t => t.1.Valuation → EffectKind.impure.toMonad d.m (toType t.2)) l
+    {l : RegionSignature d.Ty} → (T : HVector (fun t => Com d t.1 .impure t.2) l) →
+    HVector (fun t => t.1.Valuation → EffectKind.impure.toMonad d.m (HVector toType t.2)) l
   | _, .nil => HVector.nil
   | _, .cons v vs => HVector.cons (v.denote) (HVector.denote vs)
 
-def Expr.denote {ty : d.Ty} (e : Expr d Γ eff ty) (V : Valuation Γ) :
+def Expr.denote {ty} (e : Expr d Γ eff ty) (V : Valuation Γ) :
     eff.toMonad d.m (e.outContext.Valuation) :=
   match e with
   | ⟨op, ty_eq, heff, args, regArgs⟩ => do
       let argsDenote := args.map V
       let val ← EffectKind.liftEffect heff <| DialectDenote.denote op argsDenote regArgs.denote
-      return (V.snoc val).cast (by rw [← ty_eq])
+      return (V ++ val).cast (by rw [← ty_eq])
 
-def Com.denote : Com d Γ eff ty → (Γv : Valuation Γ) → eff.toMonad d.m (toType ty)
-  | .ret e, Γv     => pure (Γv e)
+def Com.denote : Com d Γ eff ty → (Γv : Valuation Γ) →
+    eff.toMonad d.m (HVector toType ty)
+  | .rets vs, Γv     => pure (vs.map Γv)
   | .var e body, V => e.denote V >>= body.denote
 end
 
@@ -462,7 +501,7 @@ end
 the output context of `com` -/
 def Com.denoteLets : (com : Com d Γ eff ty) → (Γv : Valuation Γ) →
     eff.toMonad d.m (com.outContext.Valuation)
-  | .ret _, V => pure V
+  | .rets _, V => pure V
   | .var e body, V =>
       e.denote V >>= body.denoteLets >>= fun V =>
         return V.cast (by simp [Com.outContext])
@@ -473,24 +512,14 @@ def Lets.denote [DialectSignature d] [DialectDenote d] {Γ₂}
   | .nil          => return V
   | .var lets' e  => lets'.denote V >>= e.denote
 
-/-- `denotePure` is a specialization of `denote` for pure `Lets`.
-Theorems and definitions should always be phrased in terms of the latter.
-
-However, `denotePure` behaves slighly better when it comes to congruences, since `congr` does not
-realize that `pure.toMonad d.m (Valuation _)` is just `Valuation _`, and thus a function.
-Therefore, if a goalstate is `⊢ lets.denote ... = lets.denote ...`, and `lets` is pure, then to use
-the congruence, you can do: `rw [← Lets.denotePure]; congr`
--/
-@[simp] abbrev Lets.denotePure [DialectSignature d] [DialectDenote d] :
-    Lets d Γ₁ .pure Γ₂ → Valuation Γ₁ → Valuation Γ₂ := Lets.denote
-
 section Unfoldings
 
 open EffectKind (liftEffect)
 
 omit [LawfulMonad d.m] in
 /-- Returns only the result of the current expression. -/
-def Expr.denoteOp (e : Expr d Γ eff ty) (V : Γ.Valuation) : eff.toMonad d.m ⟦ty⟧ :=
+def Expr.denoteOp (e : Expr d Γ eff ty) (V : Γ.Valuation) :
+    eff.toMonad d.m (HVector toType ty) :=
   EffectKind.liftEffect e.eff_le <| cast (by rw [← e.ty_eq]) <|
     DialectDenote.denote e.op (e.args.map V) e.regArgs.denote
 
@@ -506,7 +535,7 @@ Unfortunately, if we define `Expr.denote` in terms of the projections directly,
 the termination checker fails to prove termination. Hence, this workaround.
 -/
 theorem Expr.denote_unfold (e : Expr d Γ eff ty) :
-    e.denote = fun V => V.snoc <$> (e.denoteOp V) := by
+    e.denote = fun V => (V ++ ·) <$> (e.denoteOp V) := by
   rcases e with ⟨op, rfl, _⟩
   simp [denote, denoteOp]
 
@@ -549,26 +578,49 @@ info: some #[`Com.denote.eq_1, `Com.denote.eq_2]
 
 end Unfoldings
 
-/-! simp-lemmas about `denote` functions -/
+/-! ### Pure Denote -/
+
+/-- `denotePure` is a specialization of `denote` for pure `Lets`.
+Theorems and definitions should always be phrased in terms of the latter.
+
+However, `denotePure` behaves slighly better when it comes to congruences, since `congr` does not
+realize that `pure.toMonad d.m (Valuation _)` is just `Valuation _`, and thus a function.
+Therefore, if a goalstate is `⊢ lets.denote ... = lets.denote ...`, and `lets` is pure, then to use
+the congruence, you can do: `rw [← Lets.denotePure]; congr`
+-/
+@[simp] abbrev Lets.denotePure [DialectSignature d] [DialectDenote d] :
+    Lets d Γ₁ .pure Γ₂ → Valuation Γ₁ → Valuation Γ₂ := Lets.denote
+
+/-- Alias of `denoteOp` for pure expressions. -/
+@[simp] abbrev Expr.pdenoteOp :
+    Expr d Γ .pure ty → Γ.Valuation → (HVector toType ty) :=
+  Expr.denoteOp
+
+/-- Alias of `denoteOp` for pure expressions. -/
+@[simp] abbrev Com.pdenote :
+    Com d Γ .pure ty → Γ.Valuation → (HVector toType ty) :=
+  Com.denote
+
+/-! ### simp-lemmas about `denote` functions -/
 section Lemmas
 
 @[simp] lemma Expr.comap_denote_snocRight (e : Expr d Γ .pure ty) (V : Γ.Valuation) :
-    (Valuation.comap (e.denote V) Hom.id.snocRight) = V := by
-  funext t v; simp [Expr.denote_unfold]; rfl
+    (Valuation.comap (e.denote V) e.contextHom) = V := by
+  funext t v; simp [Expr.denote_unfold, Id.map_eq']
 
 @[simp] lemma HVector.denote_nil
-    (T : HVector (fun (t : Ctxt d.Ty × d.Ty) => Com d t.1 .impure t.2) []) :
+    (T : HVector (fun (t : Ctxt d.Ty × List d.Ty) => Com d t.1 .impure t.2) []) :
     HVector.denote T = HVector.nil := by
-  cases T; simp [HVector.denote]
+  cases T; rfl
 
 @[simp] lemma HVector.denote_cons
-    (t : Ctxt d.Ty × d.Ty) (ts : List (Ctxt d.Ty × d.Ty))
-    (a : Com d t.1 .impure t.2) (as : HVector (fun t => Com d t.1 .impure t.2) ts) :
-    HVector.denote (.cons a as) = .cons (a.denote) (as.denote) := by
-  simp [HVector.denote]
+    {t : _ × _} {ts : RegionSignature _}
+    (a : Com d t.1 .impure t.2) (as : Regions _ ts) :
+    HVector.denote (.cons a as) = .cons (a.denote) (as.denote) :=
+  rfl
 
-@[simp] lemma Com.denote_ret {eff : EffectKind} (Γ : Ctxt d.Ty) (x : Γ.Var t) :
-    (Com.ret x : Com d Γ eff t).denote = fun Γv => return (Γv x) := by
+@[simp] lemma Com.denote_rets {eff : EffectKind} (Γ : Ctxt d.Ty) (vs : HVector Γ.Var ts) :
+    (Com.rets (eff := eff) vs).denote = fun V => pure (vs.map V) :=
   rfl
 
 @[simp] lemma Com.denote_var [LawfulMonad d.m] {e : Expr d Γ eff α} :
@@ -599,16 +651,16 @@ Map a context homomorphism over a `Expr`/`Com`.
 That is, substitute variables.
 -/
 
-def Expr.changeVars (varsMap : Γ.Hom Γ') {ty : d.Ty} (e : Expr d Γ eff ty) :
+def Expr.changeVars (varsMap : Γ.Hom Γ') {ty} (e : Expr d Γ eff ty) :
     Expr d Γ' eff ty :=
   ⟨e.op, e.ty_eq, e.eff_le, e.args.map varsMap, e.regArgs⟩
 
 def Com.changeVars : Com d Γ eff ty →
     (varsMap : Γ.Hom Γ') →
     Com d Γ' eff ty
-  |  .ret e => fun varsMap => .ret (varsMap e)
+  |  .rets e => fun varsMap => .rets (e.map varsMap)
   |  .var e body => fun varsMap => .var (e.changeVars varsMap)
-      (body.changeVars (fun _ v => varsMap.snocMap v))
+      (body.changeVars (fun _ v => varsMap.append v))
 
 /-! simp-lemmas about `changeVars`-/
 section Lemmas
@@ -628,32 +680,33 @@ variable {Γ Γ' : Ctxt d.Ty} {t} (f : Γ.Hom Γ') (e : Expr d Γ eff t) (V : Γ
     (V : Γ'.Valuation)
     (f : e.outContext.Valuation → eff.toMonad d.m α) :
     (Expr.changeVars varsMap e).denote V
-      >>= (f <| Valuation.comap · varsMap.snocMap)
+      >>= (f <| Valuation.comap · varsMap.append)
     = e.denote (V.comap varsMap) >>= f := by
   simp [denote_unfold]
 
 end Lemmas
 
-@[simp] lemma Com.changeVars_ret (v : Var Γ t) :
-    (Com.ret (d:=d) (eff := eff) v).changeVars = fun (map : Γ.Hom Δ) => Com.ret (map v) := by
+@[simp] lemma Com.changeVars_rets :
+    (Com.rets (d:=d) (Γ:=Γ) (eff := eff) vs).changeVars
+    = fun (map : Γ.Hom Δ) => Com.rets (vs.map map) := by
   funext map
   simp [changeVars]
 
 @[simp] lemma Com.changeVars_var (e : Expr d Γ eff t) (body : Com d _ eff u) :
     (Com.var e body).changeVars
-    = fun (map : Γ.Hom Δ) => Com.var (e.changeVars map) (body.changeVars map.snocMap) := by
+    = fun (map : Γ.Hom Δ) => Com.var (e.changeVars map) (body.changeVars map.append) := by
   simp [changeVars]
 
 -- TODO: this is implied by simpler simp-lemmas, do we need it?
-@[simp] lemma Com.outContext_changeVars_ret (varsMap : Γ.Hom Γ') (_ : Com d Γ eff ty) :
-  ((Com.ret (d:=d) (eff := eff) v).changeVars varsMap).outContext = Γ' := by simp
+@[simp] lemma Com.outContext_changeVars_rets (varsMap : Γ.Hom Γ') (_ : Com d Γ eff ty) :
+  ((Com.rets (d:=d) (eff := eff) v).changeVars varsMap).outContext = Γ' := by simp
 
 @[simp] lemma Com.denote_changeVars
     (varsMap : Γ.Hom Γ') (c : Com d Γ eff ty) :
     (c.changeVars varsMap).denote =
     fun V => c.denote (V.comap varsMap) := by
   induction c using Com.rec' generalizing Γ' with
-  | ret x      => simp
+  | rets x      => simp [HVector.map_map]; rfl
   | var _ _ ih => simp [denote, ih]
 
 @[simp] lemma Com.denote_changeVars' (varsMap : Γ.Hom Γ') (c : Com d Γ eff ty) :
@@ -662,21 +715,40 @@ end Lemmas
 
 @[simp] def Com.outContext_changeVars_hom {map : Γ.Hom Δ} (map_inv : Δ.Hom Γ) :
     {c : Com d Γ eff ty} → Ctxt.Hom (outContext (changeVars c map)) (outContext c)
-  | .ret _        => cast (by simp) map_inv
+  | .rets _        => cast (by simp) map_inv
   | .var _ body  => cast (by simp) <|
-      Com.outContext_changeVars_hom (map := map.snocMap) map_inv.snocMap (c := body)
+      Com.outContext_changeVars_hom (map := map.append) map_inv.append (c := body)
 
-@[simp] lemma Com.denoteLets_returnVar_pure (c : Com d Γ .pure ty) (Γv : Valuation Γ) :
-    c.denoteLets Γv c.returnVar = c.denote Γv := by
+@[simp] lemma Com.denoteLets_returnVars (c : Com d Γ .pure tys) (V : Valuation Γ) :
+    c.returnVars.map (c.denoteLets V) = c.denote V := by
   induction c using Com.rec'
-  · simp; rfl
-  · rename_i a
-    simp only [denoteLets, outContext_var, Valuation.cast_rfl, Id.pure_eq',
-      Id.bind_eq', returnVar_var, a, denote]
+  case rets v  => rfl
+  case var ih => simp [denoteLets, Id.pure_eq', Id.bind_eq', ih, denote]
 
 @[simp] lemma Expr.changeVars_changeVars (e : Expr d Γ eff ty) (f : Γ.Hom Δ) (g : Δ.Hom Ξ) :
     (e.changeVars f).changeVars g = e.changeVars (f.comp g) := by
   simp [changeVars, HVector.map_map]; rfl
+
+/-! ### ChangeVars & Specific Morphisms -/
+
+lemma Expr.changeVars_castCodomain (e : Expr d Γ eff t)
+    (f : Hom Γ Δ) (h : Δ = Δ') :
+    e.changeVars (f.castCodomain h) = cast (by simp [h]) (e.changeVars f) := by
+  subst h; rfl
+
+@[simp] lemma HVector.changeVars_id {Γ : Ctxt d.Ty} (vs : HVector Γ.Var ts) :
+    vs.map Hom.id = vs := by
+  induction vs <;> simp [map, *]
+
+@[simp] lemma Expr.changeVars_id (e : Expr d Γ eff t) :
+    e.changeVars .id = e := by
+  cases e; simp [changeVars]
+
+@[simp] lemma Com.changeVars_id (c : Com d Γ eff t) :
+    c.changeVars .id = c := by
+  induction c
+  · simp
+  · simpa
 
 /-!
 ## FlatCom
@@ -686,9 +758,9 @@ An alternative representation of a program as a `Lets` with a return `Var`
 /-- `FlatCom Γ eff Δ ty` represents a program as a sequence `Lets Γ eff Δ` and a `Var Δ ty`.
 This is isomorphic to `Com Γ eff ty`, where `Δ` is `com.outContext` -/
 structure FlatCom (d : Dialect) [DialectSignature d]  (Γ_in : Ctxt d.Ty) (eff : EffectKind)
-    (Γ_out : Ctxt d.Ty) (ty : d.Ty) where
+    (Γ_out : Ctxt d.Ty) (ts : List d.Ty) where
   lets : Lets d Γ_in eff Γ_out
-  ret : Var Γ_out ty
+  rets : HVector Γ_out.Var ts
 
 --TODO: should this be a `@[simp] abbrev`, or just nuked altogether?
 /-- Denote the Lets of the FlatICom -/
@@ -696,20 +768,16 @@ def FlatCom.denoteLets (flatCom : FlatCom d Γ eff Γ_out t) (Γv : Γ.Valuation
     eff.toMonad d.m <| Γ_out.Valuation :=
   flatCom.lets.denote Γv
 
-/-- Denote the lets and the ret of the FlatCom. This is equal to denoting the Com -/
-@[simp] abbrev FlatCom.denote [DialectDenote d] (flatCom : FlatCom d Γ eff Γ_out t)
-    (Γv : Γ.Valuation) : eff.toMonad d.m (toType t) :=
-  flatCom.lets.denote Γv >>= fun Γ'v => return (Γ'v flatCom.ret)
+/-- Denote the lets and the rets of the FlatCom. This is equal to denoting the Com -/
+@[simp] abbrev FlatCom.denote [DialectDenote d]
+    (flatCom : FlatCom d Γ eff Γ_out ts)
+    (V : Γ.Valuation) : eff.toMonad d.m (HVector toType ts) :=
+  flatCom.lets.denote V >>= (return flatCom.rets.map ·)
 
 theorem FlatCom.denoteLets_eq [DialectDenote d] (flatCom : FlatCom d Γ eff Γ_out t) :
     flatCom.denoteLets = fun Γv => flatCom.lets.denote Γv := by
   funext Γv
   simp [denoteLets]
-
-theorem FlatCom.denote_eq [DialectDenote d] (flatCom : FlatCom d Γ eff Γ_out t) :
-    flatCom.denote = fun Γv => flatCom.lets.denote Γv >>= fun Γ'v => return (Γ'v flatCom.ret) := by
-  funext Γv
-  simp [denote]
 
 /-!
 ## casting of expressions and purity
@@ -734,7 +802,7 @@ phrased more generically -/
 def Com.changeEffect {eff₁ eff₂ : EffectKind} (h : eff₁ ≤ eff₂) :
     Com d Γ eff₁ t → Com d Γ eff₂ t := fun com =>
   Com.rec' (motive := @fun Γ _ => eff₁ ≤ eff₂ → Com d Γ eff₂ t)
-    /- ret v -/       (fun v _h               => ret v)
+    /- rets v -/       (fun v _h               => rets v)
     /- var e body -/ (fun e _body castBody h => var (e.changeEffect h) (castBody h))
     com h
 
@@ -763,12 +831,12 @@ but for some reason doing so causes `Lets.castPureToEff_var` to no longer be def
 
 /-- A wrapper around `Com.var` that allows for a pure expression to be added to an otherwise
 impure program, using `Expr.castPureToEff` -/
-def Com.letPure (e : Expr d Γ .pure t) (body : Com d (Γ.snoc t) eff u) : Com d Γ eff u :=
+def Com.letPure (e : Expr d Γ .pure t) (body : Com d (e.outContext) eff u) : Com d Γ eff u :=
   body.var (e.castPureToEff eff)
 
 /-- `letSup e body` allows us to combine an expression and body with different effects,
 by returning a `Com` whose effect is their join/supremum -/
-def Com.letSup (e : Expr d Γ eff₁ t) (body : Com d (Γ.snoc t) eff₂ u) :
+def Com.letSup (e : Expr d Γ eff₁ t) (body : Com d (e.outContext) eff₂ u) :
     Com d Γ (eff₁ ⊔ eff₂) u :=
   Com.var (e.changeEffect <| by simp) (body.changeEffect <| by simp)
 
@@ -780,7 +848,7 @@ section Lemmas
     (e.castPureToEff eff).args = cast (by simp) e.args := by
   cases e; cases eff <;> rfl
 
-@[simp] lemma Com.castPureToEff_ret : (ret v : Com d Γ .pure ty).castPureToEff eff = ret v := rfl
+@[simp] lemma Com.castPureToEff_rets : (rets v : Com d Γ .pure ty).castPureToEff eff = rets v := rfl
 @[simp] lemma Com.castPureToEff_var {com : Com d _ .pure ty} {e : Expr d Γ _ eTy} :
     (var e com).castPureToEff eff = var (e.castPureToEff eff) (com.castPureToEff eff) := rfl
 
@@ -792,16 +860,21 @@ section Lemmas
 
 @[simp] lemma Com.outContext_castPureToEff {com : Com d Γ .pure ty} :
     (com.castPureToEff eff).outContext = com.outContext := by
-  induction com using Com.rec' <;> simp [*]
+  induction com <;> simp [*]
 
 /-- `castPureToEff` does not change the size of a `Com` -/
 @[simp] lemma Com.size_castPureToEff {com : Com d Γ .pure ty} :
     (com.castPureToEff eff).size = com.size := by
-  induction com using Com.rec' <;> simp [*]
+  induction com <;> simp [*]
 
-@[simp] lemma Com.returnVar_castPureToEff {com : Com d Γ .pure ty} :
-    (com.castPureToEff eff).returnVar = com.returnVar.castCtxt (by simp) := by
-  induction com using Com.rec' <;> simp_all
+/-- `castPureToEff` does not change the number of bvars of a `Com` -/
+@[simp] lemma Com.bvars_castPureToEff {com : Com d Γ .pure ty} :
+    (com.castPureToEff eff).bvars = com.bvars := by
+  induction com <;> simp [*]
+
+@[simp] lemma Com.returnVars_castPureToEff (eff : _) (com : Com d Γ .pure tys) :
+    (com.castPureToEff eff).returnVars = com.returnVars.map (fun _ v => v.castCtxt (by simp)) := by
+  induction com <;> simp_all
 
 /-! denotations of `castPureToEff` -/
 
@@ -863,7 +936,7 @@ end toPureLemmas
 
 theorem Expr.denote_pure {e : Expr d Γ .pure ty} :
     e.denote = fun (V : Valuation Γ) =>
-      return (V.snoc <| e.denoteOp V) := by
+      return ((V ++ · : HVector _ _ → _) <| e.denoteOp V) := by
   funext V t v
   simp [denote_unfold]; rfl
 
@@ -889,10 +962,9 @@ equivalent to the return value of the inserted program `newCom`, then the denota
 after insertion agrees with the original zipper. -/
 section DenoteInsert
 
-@[simp] lemma Expr.denote_snoc (e : Expr d Γ .pure t) (V : Γ.Valuation) (v : Γ.Var u) :
-    e.denote V v.toSnoc = V v := by
-  simp only [denote_unfold]
-  apply Valuation.snoc_toSnoc
+@[simp] lemma Expr.denote_appendInl (e : Expr d Γ .pure t) (V : Γ.Valuation) (v : Γ.Var u) :
+    e.denote V v.appendInl = V v := by
+  simp [denote_unfold, Id.map_eq']
 
 /-- Denoting any of the free variables of a program through `Com.denoteLets` just returns the
 assignment of that variable in the input valuation -/
@@ -903,40 +975,17 @@ assignment of that variable in the input valuation -/
   · simp; rfl
   case var e body ih =>
     rw [outContextHom_var]
-    simp only [Ctxt.Hom.unSnoc_apply, denoteLets_var]
-    show body.denoteLets (e.denote V) _ = _
-    simp [ih]
-
+    simp [Id.bind_eq', Hom.comp, ih]
 
 @[simp] lemma Ctxt.Valuation.comap_outContextHom_denoteLets {com : Com d Γ .pure ty} {V} :
     Valuation.comap (com.denoteLets V) com.outContextHom = V := by
   unfold comap; simp
-
--- TODO: This theorem is currently not used yet. The hope is that it might replace/simplify the
---       subtype reasoning (`denoteIntoSubtype`) currently used when reasoning about `matchVar`
--- theorem Zipper.denote_insertPureCom_eq_of {zip : Zipper d Γ_in eff Γ_mid ty₁}
---     {newCom : Com d _ _ newTy} {V_in : Valuation Γ_in} [LawfulMonad d.m]
---     (h : ∀ V_mid ∈ Functor.supp (zip.top.denote V_in),
---             newCom.denote V_mid = V_mid v) :
---     (zip.insertPureCom v newCom).denote V_in = zip.denote V_in := by
---   rcases zip with ⟨lets, com⟩
---   simp only [denote_insertPureCom, Valuation.comap_with,
---   Valuation.comap_outContextHom_denoteLets, Com.denoteLets_returnVar_pure,
---   denote_mk]
---   unfold Valuation.reassignVar
---   congr; funext V_mid; congr
---   funext t' v'
---   simp only [dite_eq_right_iff, forall_exists_index]
---   rintro rfl rfl
---   simpa using h _ (sorry : V_mid ∈ Functor.supp (lets.denote V_in))
 
 end DenoteInsert
 
 /-!
 ### Inserting multiple programs with `Zipper.foldInsert`
 -/
-
--- def Zipper.foldInsert
 
 /-!
 ## Random Access for `Lets`
@@ -948,41 +997,73 @@ so long as the binding's operation is pure
 without adjusting variables, assuming that this expression has a pure operation.
 If the expression has an impure operation, or there is no binding corresponding to `v`
 (i.e., `v` comes from `Γ_in`), return `none` -/
-def Lets.getPureExprAux {Γ₁ Γ₂ : Ctxt d.Ty} {t : d.Ty} : Lets d Γ₁ eff Γ₂ → (v : Var Γ₂ t) →
-    Option (Expr d (Γ₂.dropUntil v) .pure t)
+def Lets.getPureExprAux {Γ₁ Γ₂ : Ctxt d.Ty} {t} : Lets d Γ₁ eff Γ₂ → (v : Var Γ₂ t) →
+    Option (Σ ts, (Var ⟨ts⟩ t) × Expr d (Γ₂.dropUntil v) .pure ts)
   | .nil, _ => none
-  | .var lets e, v => by
-    cases v using Var.casesOn with
-      | toSnoc v => exact (Lets.getPureExprAux lets v)
-      | last => exact e.toPure?
+  | .var (Γ_out := Γ_out) (t := t) lets e, v => by
+    cases v using Var.appendCases with
+    | left v =>
+        apply cast ?_ <| Lets.getPureExprAux lets v
+        simp
+    | right v =>
+        have h : Γ_out ++ (t.drop <| v.1 + 1) = e.outContext.dropUntil v.appendInr := by simp
+        let f := Hom.castCodomain h <| .appendCodomain .id
+        exact e.toPure?.map (fun e => ⟨_, v, e.changeVars f⟩)
 
 /-- Get the `Expr` that a var `v` is assigned to in a sequence of `Lets`.
 The variables are adjusted so that they are variables in the output context of a lets,
 not the local context where the variable appears. -/
 def Lets.getPureExpr {Γ₁ Γ₂ : Ctxt d.Ty} (lets : Lets d Γ₁ eff Γ₂) {t : d.Ty} (v : Var Γ₂ t) :
-    Option (Expr d Γ₂ .pure t) :=
-  Expr.changeVars Ctxt.dropUntilHom <$> getPureExprAux lets v
+    Option (Σ ts, (Var ⟨ts⟩ t) × Expr d Γ₂ .pure ts) :=
+  (getPureExprAux lets v).map fun ⟨_, v, e⟩ =>
+    ⟨_, v, e.changeVars Ctxt.dropUntilHom⟩
 
 @[simp] lemma Lets.getPureExpr_nil : getPureExpr (.nil : Lets d Γ eff Γ) v = none := rfl
 
-@[simp] lemma Lets.getPureExpr_var_last (lets : Lets d Γ_in eff Γ_out)
-    (e : Expr d Γ_out eff ty) :
-    getPureExpr (lets.var e) (Var.last ..)
-    = (Expr.changeVars <| Ctxt.Hom.id.snocRight) <$> e.toPure? := by
-  rfl
-@[simp] lemma Lets.getPureExprAux_var_toSnoc (lets : Lets d Γ_in eff Γ_out)
-    (e : Expr d Γ_out eff ty₁) (v : Var Γ_out ty₂) :
-    getPureExprAux (lets.var e) (v.toSnoc) = getPureExprAux lets v :=
-  rfl
+@[simp] lemma Lets.getPureExpr_var_appendInr (lets : Lets d Γ_in eff Γ_out)
+    (e : Expr d Γ_out eff ty) (v : Var ⟨ty⟩ u) :
+    getPureExpr (lets.var e) v.appendInr
+    = e.toPure?.map (fun e => ⟨_, v, e.changeVars <| e.contextHom⟩) := by
+  simp only [getPureExpr, getPureExprAux, Ctxt.getElem?_ofList, Var.appendCases_appendInr,
+    Option.map_map]
+  congr 1
+  funext e
+  simp only [Expr.changeVars_changeVars, Function.comp]
+  congr 3
+  funext _ v'
+  apply Subtype.eq
+  have := v.val_lt
+  simp; grind
 
-@[simp] lemma Lets.getPureExpr_var_toSnoc (lets : Lets d Γ_in eff Γ_out) (e : Expr d Γ_out _ ty₁)
+
+@[simp] lemma Lets.getPureExprAux_var_appendInl (lets : Lets d Γ_in eff Γ_out)
+    (e : Expr d Γ_out eff ty₁) (v : Var Γ_out ty₂) :
+    getPureExprAux (lets.var e) v.appendInl
+    = (getPureExprAux lets v).map fun ⟨_, w, e⟩ =>
+        ⟨_, w, e.changeVars <| Hom.id.castCodomain (by simp)⟩ := by
+  simp [getPureExprAux]
+  match lets.getPureExprAux v with
+  | none =>
+    simp only [Option.map_none, cast_eq_iff_heq]
+    congr
+    simp
+  | some ⟨_, _, e⟩ =>
+    simp only [Option.map_some, cast_eq_iff_heq]
+    congr 3 <;> simp [Expr.changeVars_castCodomain]
+
+@[simp] lemma Lets.getPureExpr_var_appendInl (lets : Lets d Γ_in eff Γ_out) (e : Expr d Γ_out _ ty₁)
     (v : Var Γ_out ty₂):
-    getPureExpr (lets.var e) (v.toSnoc)
-    = (Expr.changeVars <| Ctxt.Hom.id.snocRight) <$> (getPureExpr lets v) := by
-  simp only [getPureExpr, Ctxt.dropUntilHom_toSnoc,
-    getPureExprAux_var_toSnoc, Option.map_eq_map, Option.map_map, Function.comp_def,
-    Expr.changeVars_changeVars]
-  rfl
+    getPureExpr (lets.var e) (v.appendInl)
+    = (fun ⟨_, w, e'⟩ => ⟨_, w,  e'.changeVars <| e.contextHom⟩) <$> (getPureExpr lets v) := by
+  simp only [getPureExpr, getPureExprAux_var_appendInl, Option.map_eq_map, Option.map_map]
+  congr 1
+  funext ⟨_, e⟩
+  simp only [Function.comp_apply, Expr.changeVars_changeVars, Sigma.mk.injEq, heq_eq_eq, true_and]
+  congr 2
+  funext t v
+  apply Subtype.eq
+  simp [Hom.castCodomain, Hom.comp, Ctxt.dropUntilHom, Ctxt.dropUntilDiff, Ctxt.Diff.toHom, Var.appendInl]
+  omega
 
 /-!
 ## Mapping
@@ -992,21 +1073,21 @@ We can map between different dialects
 section Map
 
 def RegionSignature.map (f : Ty → Ty') : RegionSignature Ty → RegionSignature Ty' :=
-  List.map fun ⟨Γ, ty⟩ => (Γ.map f, f ty)
+  List.map fun ⟨Γ, ty⟩ => (Γ.map f, ty.map f)
 
 instance : Functor RegionSignature where
   map := RegionSignature.map
 
 def Signature.map (f : Ty → Ty') : Signature Ty → Signature Ty' :=
   fun sig => {
-    sig    := sig.sig.map f
-    regSig := sig.regSig.map f
-    outTy  := f sig.outTy
+    sig         := sig.sig.map f
+    regSig      := sig.regSig.map f
+    returnTypes := sig.returnTypes.map f
   }
 
 instance : Functor Signature where
-  map := fun f ⟨sig, regSig, outTy, effKind⟩ =>
-    ⟨f <$> sig, f <$> regSig, f outTy, effKind⟩
+  map := fun f ⟨sig, regSig, returnTypes, effKind⟩ =>
+    ⟨f <$> sig, f <$> regSig, f <$> returnTypes, effKind⟩
 
 /-- A dialect morphism consists of a map between operations and a map between types,
 such that the signature of operations is respected -/
@@ -1025,9 +1106,9 @@ def DialectMorphism.preserves_regSig (op : d.Op) :
     DialectSignature.regSig (f.mapOp op) = (DialectSignature.regSig op).map f.mapTy := by
   simp only [DialectSignature.regSig, Function.comp_apply, f.preserves_signature]; rfl
 
-def DialectMorphism.preserves_outTy (op : d.Op) :
-    DialectSignature.outTy (f.mapOp op) = f.mapTy (DialectSignature.outTy op) := by
-  simp only [DialectSignature.outTy, Function.comp_apply, f.preserves_signature]; rfl
+def DialectMorphism.preserves_returnTypes (op : d.Op) :
+    DialectSignature.returnTypes (f.mapOp op) = (DialectSignature.returnTypes op).map f.mapTy := by
+  simp only [DialectSignature.returnTypes, Function.comp_apply, f.preserves_signature]; rfl
 
 theorem DialectMorphism.preserves_effectKind (op : d.Op) :
     DialectSignature.effectKind (f.mapOp op) = DialectSignature.effectKind op := by
@@ -1035,19 +1116,25 @@ theorem DialectMorphism.preserves_effectKind (op : d.Op) :
 
 mutual
 
-def Com.changeDialect : Com d Γ eff ty → Com d' (f.mapTy <$> Γ) eff (f.mapTy ty)
-  | .ret v          => .ret v.toMap
-  | .var body rest => .var body.changeDialect rest.changeDialect
+def Com.changeDialect : Com d Γ eff ty → Com d' (f.mapTy <$> Γ) eff (f.mapTy <$> ty)
+  | .rets vs        => .rets <| vs.map' f.mapTy (fun _ v => v.toMap)
+  | .var body rest =>
+      let rest :=
+        rest.changeDialect.changeVars <|
+          Hom.id.castCodomain (by simp)
+      .var body.changeDialect rest
+termination_by com => sizeOf com
 
-def Expr.changeDialect : Expr d Γ eff ty → Expr d' (Γ.map f.mapTy) eff (f.mapTy ty)
+def Expr.changeDialect : Expr d Γ eff ty → Expr d' (Γ.map f.mapTy) eff (f.mapTy <$> ty)
   | ⟨op, Eq.refl _, effLe, args, regs⟩ => ⟨
       f.mapOp op,
-      (f.preserves_outTy _).symm,
+      (f.preserves_returnTypes _).symm,
       f.preserves_effectKind _ ▸ effLe,
       f.preserves_sig _ ▸ args.map' f.mapTy fun _ => Var.toMap (f:=f.mapTy),
       f.preserves_regSig _ ▸
         HVector.changeDialect regs
     ⟩
+termination_by e => sizeOf e
 
 /-- Inline of `HVector.map'` for the termination checker -/
 def HVector.changeDialect : ∀ {regSig : RegionSignature d.Ty},
@@ -1055,22 +1142,28 @@ def HVector.changeDialect : ∀ {regSig : RegionSignature d.Ty},
     → HVector (fun t => Com d' t.fst eff t.snd) (f.mapTy <$> regSig : RegionSignature _)
   | _, .nil        => .nil
   | t::_, .cons a as  => .cons a.changeDialect (HVector.changeDialect as)
+termination_by _ vs => sizeOf vs
 
 end
 
 def Lets.changeDialect : Lets d Γ_in eff Γ_out → Lets d' (f.mapTy <$> Γ_in) eff (f.mapTy <$> Γ_out)
   | nil => nil
-  | var body e => var (changeDialect body) (e.changeDialect f)
+  | var body e =>
+      cast (by simp) <| var (changeDialect body) (e.changeDialect f)
 
 section Lemmas
 
-@[simp] lemma Com.changeDialect_ret (f : DialectMorphism d d') (v : Var Γ t) :
-    Com.changeDialect f (Com.ret v : Com d Γ eff t) = Com.ret v.toMap := by
+@[simp] lemma Com.changeDialect_rets (f : DialectMorphism d d') (vs) :
+    Com.changeDialect f (Com.rets vs : Com d Γ eff t)
+    = Com.rets (vs.map' f.mapTy (fun _ v => v.toMap)) := by
   cases eff <;> simp [changeDialect]
 
 @[simp] lemma Com.changeDialect_var (f : DialectMorphism d d')
     (e : Expr d Γ eff t) (body : Com d _ eff u) :
-    (Com.var e body).changeDialect f = Com.var (e.changeDialect f) (body.changeDialect f) := by
+    (Com.var e body).changeDialect f
+    = have h := by simp
+      Com.var (e.changeDialect f)
+      <| (body.changeDialect f).changeVars (Hom.id.castCodomain h) := by
   simp only [changeDialect]
 
 @[simp] lemma HVector.changeDialect_nil {eff : EffectKind} (f : DialectMorphism d d') :
@@ -1087,7 +1180,7 @@ end Map
 /-- Add a `Com` to the end of a sequence of lets -/
 def Lets.addComToEnd {Γ_out} {eff} (lets : Lets d Γ_in eff Γ_out) :
       (com : Com d Γ_out eff ty) → Lets d Γ_in eff com.outContext
-  | Com.ret _       => lets
+  | Com.rets _       => lets
   | Com.var e body => addComToEnd (Lets.var lets e) body
 
 /-- The let-bindings of a program -/
@@ -1095,19 +1188,19 @@ def Com.toLets (com : Com d Γ eff t) : Lets d Γ eff com.outContext :=
   Lets.nil.addComToEnd com
 
 /-- Convert a `Com` into a `FlatCom` -/
-def Com.toFlatCom {t : d.Ty} (com : Com d Γ .pure t) : FlatCom d Γ .pure com.outContext t :=
-  ⟨com.toLets, com.returnVar⟩
+def Com.toFlatCom {ts} (com : Com d Γ .pure ts) : FlatCom d Γ .pure com.outContext ts :=
+  ⟨com.toLets, com.returnVars⟩
 
 section Lemmas
 
 /-! #### Basic Lemmas -/
 
-@[simp] lemma Lets.addComToEnd_ret {lets : Lets d Γ_in eff Γ_out} :
-    addComToEnd lets (.ret v : Com d Γ_out eff t) = lets             := by simp [addComToEnd]
+@[simp] lemma Lets.addComToEnd_rets {lets : Lets d Γ_in eff Γ_out} :
+    addComToEnd lets (.rets v : Com d Γ_out eff t) = lets             := by simp [addComToEnd]
 @[simp] lemma Lets.addComToEnd_var {lets : Lets d Γ_in eff Γ_out} {com : Com d _ eff t} :
     addComToEnd lets (Com.var e com) = addComToEnd (lets.var e) com := by simp [addComToEnd]
 
-@[simp] lemma Com.toLets_ret : toLets (ret v : Com d Γ eff t) = .nil := by simp [toLets]
+@[simp] lemma Com.toLets_rets : toLets (rets v : Com d Γ eff t) = .nil := by simp [toLets]
 
 /-! ### castPureToEff -/
 
@@ -1116,7 +1209,7 @@ section Lemmas
     (lets.castPureToEff eff).addComToEnd (com.castPureToEff eff)
     = cast (by simp) ((lets.addComToEnd com).castPureToEff eff) := by
   induction com using Com.rec'
-  case ret => simp
+  case rets => simp
   case var ih =>
     simp only [Com.castPureToEff_var, Com.outContext_var, addComToEnd_var,
       ← Lets.castPureToEff_var, ih]
@@ -1137,10 +1230,10 @@ section Lemmas
         return Vbody
       ) := by
   induction com
-  case ret => simp [Com.denoteLets]
+  case rets => simp [Com.denoteLets]
   case var ih => simp [addComToEnd, ih, denote_var]
 
-@[simp] lemma Com.denoteLets_ret : (.ret v : Com d Γ eff t).denoteLets = fun V => pure V := by
+@[simp] lemma Com.denoteLets_rets : (.rets v : Com d Γ eff t).denoteLets = fun V => pure V := by
   funext V; simp [denoteLets]
 
 theorem Com.denoteLets_eq {com : Com d Γ eff t} : com.denoteLets = com.toLets.denote := by
@@ -1169,28 +1262,39 @@ def HVector.toVarSet : {l : List d.Ty} → (T : HVector (Var Γ) l) → VarSet �
 def HVector.vars {l : List d.Ty} (T : HVector (Var Γ) l) : VarSet Γ :=
   T.foldl (fun _ s a => insert ⟨_, a⟩ s) ∅
 
+mutual
+
 --TODO: find a name that better encapsulates that it's the *transitive* closure
 /-- The free variables of `lets` that are (transitively) referred to by some variable `v`.
 Also known as the uses of var. -/
 def Lets.vars : Lets d Γ_in eff Γ_out → Var Γ_out t → VarSet Γ_in
   | .nil, v => VarSet.ofVar v
   | .var lets e, v => by
-      cases v using Var.casesOn with
-      | toSnoc v => exact lets.vars v
-      | last => exact (e.args.vars).biUnion (fun v => lets.vars v.2)
+      cases v using Var.appendCases with
+      | left v => exact lets.vars v
+      | right _ => exact lets.varsOfVec e.args
 
+def Lets.varsOfVec (lets : Lets d Γ_in eff Γ_out) (vs : HVector Γ_out.Var ts) :
+    VarSet Γ_in :=
+  (vs.vars).biUnion (fun v => lets.vars v.2)
+
+end
 
 /-- `com.vars` is the set of free variables from `Γ` that are (transitively) used by the return
 variable of `com` -/
-def Com.vars : Com d Γ .pure t → VarSet Γ :=
-  fun com => com.toFlatCom.lets.vars com.toFlatCom.ret
+def Com.vars (com : Com d Γ eff ts) : VarSet Γ :=
+  com.toLets.varsOfVec com.returnVars
 
-theorem Lets.vars_var_eq {lets : Lets d Γ_in eff Γ_out}
-  {t: d.Ty} {e : Expr d Γ_out eff t}
-  {w : ℕ} {tw : d.Ty} {wh : Γ_out[w]? = some tw} :
-  Lets.vars (Lets.var lets e) ⟨w + 1, by simpa [Ctxt.snoc] using wh⟩ =
-  Lets.vars lets ⟨w, wh⟩ := by simp [Lets.vars]
+section Lemmas
 
+@[simp] lemma Com.vars_toLets (com : Com d Γ eff t) :
+    com.toLets.varsOfVec com.returnVars = com.vars := rfl
+
+@[simp] lemma Lets.vars_var {lets : Lets d Γ_in eff Γ_out}
+    {t} {e : Expr d Γ_out eff t} {w : Γ_out.Var u} :
+    Lets.vars (Lets.var lets e) w.appendInl
+    = Lets.vars lets w := by
+  simp [Lets.vars]
 
 @[simp] lemma HVector.vars_nil :
     (HVector.nil : HVector (Var Γ) ([] : List d.Ty)).vars = ∅ := by
@@ -1232,17 +1336,47 @@ theorem HVector.map_eq_of_eq_on_vars {A : d.Ty → Type*}
       apply h
       simp_all
 
+end Lemmas
 
-
+/-!
+## Misc
+-/
 section TypeProjections
 variable {d : Dialect} [DialectSignature d] {Γ : Ctxt d.Ty} {eff : EffectKind} {t : d.Ty}
 
-def Com.getTy : Com d Γ eff t → Type := fun _ => d.Ty
-def Com.ty : Com d Γ eff t → d.Ty := fun _ => t
-def Com.ctxt : Com d Γ eff t → Ctxt d.Ty := fun _ => Γ
+def Com.getTy : Com d Γ eff [t] → Type := fun _ => d.Ty
+def Com.ty : Com d Γ eff [t] → d.Ty := fun _ => t
+def Com.ctxt : Com d Γ eff [t] → Ctxt d.Ty := fun _ => Γ
 
-def Expr.getTy : Expr d Γ eff t → Type := fun _ => d.Ty
-def Expr.ty : Expr d Γ eff t → d.Ty := fun _ => t
-def Expr.ctxt : Expr d Γ eff t → Ctxt d.Ty := fun _ => Γ
+def Expr.getTy : Expr d Γ eff [t] → Type := fun _ => d.Ty
+def Expr.ty : Expr d Γ eff [t] → d.Ty := fun _ => t
+def Expr.ctxt : Expr d Γ eff [t] → Ctxt d.Ty := fun _ => Γ
 
 end TypeProjections
+
+/-!
+## Compatibility Namespaces
+-/
+section Compat
+
+def Com.ret {Γ : Ctxt d.Ty} {ty : d.Ty} {eff : EffectKind} : Γ.Var ty → Com d Γ eff [ty] :=
+  (Com.rets [·]ₕ)
+
+/-!
+`open LeanMLIR.SingleReturnCompat` will bring an alias for `Com` & `Expr` into
+scope which has only a single return type.
+-/
+namespace LeanMLIR.SingleReturnCompat
+variable (d) [DialectSignature d]
+
+nonrec abbrev Com  : Ctxt d.Ty → EffectKind → d.Ty → Type := (Com d · · [·])
+nonrec abbrev Expr : Ctxt d.Ty → EffectKind → d.Ty → Type := (Expr d · · [·])
+
+variable {d} {Γ : Ctxt d.Ty} {eff : EffectKind} {t : d.Ty}
+
+nonrec abbrev Com.var : Expr d Γ eff t → Com d (Γ.snoc t) eff β → Com d Γ eff β :=
+  (Com.var · ·)
+
+end LeanMLIR.SingleReturnCompat
+
+end Compat
